Strict eta expanded constructors (#680)
* Refine evaluation to maintain that constructors are never over-applied

* Show the new EtaInd principle, ensuring strict eta-expansion of constructors during evaluation. Stripping preserves this.

* Move a lemma to its right place, and avoid accidental dependency on ExpandLetsCorrectness in extracted code

(cherry picked from commit 11bc545a474a0bd5db2d0dda3e86232c87898363)

erasure/theories/EGlobalEnv.v
@@ -88,6 +88,10 @@ Definition inductive_isprop_and_pars Σ ind :=
   '(mdecl, idecl) <- lookup_inductive Σ ind ;;
   ret (idecl.(ind_propositional), mdecl.(ind_npars)).
 
+Definition constructor_isprop_pars_decl Σ ind c :=
+  '(mdecl, idecl, cdecl) <- lookup_constructor Σ ind c ;;
+  ret (idecl.(ind_propositional), mdecl.(ind_npars), cdecl).
+  
 Definition closed_decl (d : EAst.global_decl) := 
   match d with
   | EAst.ConstantDecl cb => 
